src/ExpandWhens_rewritten.v
@@ -94,6 +94,7 @@ induction pp.
   1,2: destruct (code_type_find_vm_widths (Gtyp f) s vm) as [[[newgt| |] _]|] ; try done.
   1,2: rewrite -H1 ; clear H1 newgt.
   1,2: destruct (ports_tmap pp vm) ; last by trivial.
+  1,2: destruct (CEP.find s t) ; first by trivial.
   1,2: intro.
   1,2: destruct (v == s) eqn: Hvs.
   1,3: rewrite CEP.Lemmas.find_add_eq ; first (by apply H) ;
@@ -1194,6 +1195,7 @@ induction pp.
   1,2: destruct (code_type_find_vm_widths (Gtyp gt) v vm) as [[[newgt| |]]|] ; try done.
   1,2: rewrite -H0 ; clear H0 newgt n.
   1,2: destruct (ports_tmap pp vm) as [pmap|]; last by trivial.
+  1,2: destruct (CEP.find v pmap) ; first by trivial.
   1,2: destruct (ExpandPort_fun pp) as [[temp_conn_map temp_scope]|]; last by trivial.
   1,2: intro.
   1,2: destruct (y == v) eqn: Hyv.
@@ -1224,69 +1226,151 @@ induction pp ; first by (simpl ; intros ; destruct H1 ; rewrite H2 ; reflexivity
 intros.
 generalize (ports_tmap_preserves_fully_inferred vm (a :: pp) H) ; intro.
 simpl ports_have_fully_inferred_ground_types in H.
+generalize (ports_tmap_names vm pp) ; intro.
+generalize (ports_tmap_uniq vm (a :: pp)) ; intro.
 destruct (ports_tmap (a :: pp) vm) as [pmap|] eqn: Hpmap ; last by trivial.
 intros.
 simpl ports_tmap in Hpmap.
-destruct H2 as [vm' [ct' [H2 H3]]].
+destruct H4 as [vm' [ct' [H4 H5]]].
 assert (submap vm' vm /\ submap ct' ct)
       by (apply Sem_frag_ports_submap with (pp := [:: a]) (tmap := tmap) ;
           simpl ; exists vm', ct' ;
-          split ; last (by exact H3) ; split ; reflexivity).
-unfold Sem_frag_port in H3.
+          split ; last (by exact H5) ; split ; reflexivity).
+unfold Sem_frag_port in H5.
 destruct (ExpandPort_fun (a :: pp)) as [[new_conn_map new_scope]|] eqn: Hexpand ; last by trivial.
 simpl ExpandPort_fun in Hexpand.
 destruct a as [p [gt| |]|p [gt| |]] ; try done.
-1,2: move /andP : H => [H H5].
-1,2: specialize (IHpp vm' ct' H5).
+1,2: move /andP : H => [H H7].
+1,2: specialize (IHpp vm' ct' H7).
 1,2: destruct (ExpandPort_fun pp) as [[temp_conn_map temp_scope]|] ; last by discriminate Hexpand.
 1,2: injection Hexpand ; clear Hexpand ; intros _ Hexpand ;
      rewrite -Hexpand ; clear new_conn_map new_scope temp_scope Hexpand.
 1,2: generalize (fully_inferred_does_not_change gt p vm H) ; intro.
 1,2: destruct (code_type_find_vm_widths (Gtyp gt) p vm) as [[[gt'| |] _]|] ; try by done.
-1,2: rewrite -H6 in Hpmap ; clear gt' H6.
+1,2: rewrite -H8 in Hpmap ; clear gt' H8.
 1,2: destruct (ports_tmap pp vm) as [pmap'|] eqn: Hports_tmap ; last by done.
-1,2: injection Hpmap ; clear Hpmap ; intro Hpmap.
-1,2: rewrite -Hpmap in H0, H1 ; clear pmap Hpmap.
 1,2: specialize (H1 p).
-1,2: rewrite CEP.Lemmas.find_add_eq in H1 ; last by rewrite /CEP.SE.eq //.
-1,2: rewrite H1 in H3.
-1,2: simpl size_of_ftype in H3 ; simpl list_rhs_type_p in H3.
-(* First goal: we use proj2 (proj2 H3) and IHpp to prove the result.
+1,2: destruct (CEP.find p pmap') eqn: Hfindp' ; try by done.
+1,2: destruct H1 as [H1 _].
+1,2: destruct (CEP.find p pmap') eqn: Hfindp' ; first by done.
+1,2: injection Hpmap ; clear Hpmap ; intro Hpmap.
+1,2: rewrite -Hpmap in H0, H3 ; clear pmap Hpmap.
+1,2: generalize (H3 p) ; intro.
+1,2: rewrite CEP.Lemmas.find_add_eq in H8 ; last by rewrite /CEP.SE.eq //.
+1,2: rewrite H8 in H5.
+1,2: simpl size_of_ftype in H5 ; simpl list_rhs_type_p in H5.
+(* First goal: we use proj2 (proj2 H5) and IHpp to prove the result.
    We only need to prove that ports_tmap pp vm' is Some pmap and is a submap of tmap;
-   that should be possible to prove by using the other parts of H3,
+   that should be possible to prove by using the other parts of H5,
    which state that vm and vm' are almost the same, so we finally get
    ports_tmap pp vm is basically CEP.Equal to ports_tmap pp vm'. *)
-* destruct H3 as [H3 [H6 H7]].
+* destruct H5 as [_ [H9 H10]].
+  (*specialize (H5 0) ; rewrite /List.nth_error add0n nat_of_binK -surjective_pairing in H5.*)
   intro.
-  specialize (H7 y).
-  rewrite -H7 ; destruct H4 as [H4 _] ; clear ct H7.
-
-assert (ports_tmap pp vm' = ports_tmap pp vm).
-      clear -H3 H4.
-      revert H4.
-      induction pp ;
-            first by (unfold ports_tmap ; reflexivity).
-      intro ; simpl ports_tmap.
-      simpl ports_have_fully_inferred_ground_types in H4.
-      destruct a as [p0 [gt0| |]|p0 [gt0| |]] ; try done.
-      1,2: move /andP : H4 => [H H4].
-      1,2: specialize (IHpp H4).
-      1,2: rewrite IHpp.
-      1,2: generalize (fully_inferred_does_not_change gt0 p0 vm' H) ; intro.
-      1,2: generalize (fully_inferred_does_not_change gt0 p0 vm H) ; intro.
-      1,2: destruct (code_type_find_vm_widths (Gtyp gt0) p0 vm') as [[[gt0''| |] _]|] ; try by done.
-      1,3: rewrite -H0 ; clear gt0'' H0.
-      1,2,3,4: destruct (code_type_find_vm_widths (Gtyp gt0) p0 vm) as [[[gt0'| |] _]|] ; try by done.
-      1,3: rewrite -H1 ; clear gt0' H1.
-      1,2: reflexivity.
+  specialize (H10 y).
+  rewrite -H10 ; destruct H6 as [H6 _] ; clear ct H10.
+  assert (ports_tmap pp vm' = ports_tmap pp vm).
+        clear -H2 H7 H9.
+        revert H2 H7.
+        induction pp ;
+              first by (unfold ports_tmap ; reflexivity).
+        intros ; simpl ports_tmap.
+        simpl ports_have_fully_inferred_ground_types in H7.
+        destruct a as [p0 [gt0| |]|p0 [gt0| |]] ; try done.
+        1,2: simpl uniq in H2 ; move /andP : H2 => [H21 /andP [_ H23]].
+        1,2: rewrite in_cons negb_or in H21.
+        1,2: move /andP : H21 => [H21 H22].
+        1,2: move /andP : H7 => [H H7].
+        1,2: simpl uniq in IHpp.
+        1,2: rewrite H22 H23 andTb in IHpp.
+        1,2: specialize (IHpp is_true_true H7).
+        1,2: rewrite IHpp.
+        1,2: assert (CEP.find p0 vm' = CEP.find p0 vm)
+              by (specialize (H9 p0.1 p0.2) ;
+                  rewrite add1n -surjective_pairing in H9 ;
+                  specialize (N.eq_dec p0.1 p.1) ; intro ;
+                  destruct H0 ; last (by apply H9 ; left ; exact n) ;
+                  destruct (Nat.compare_spec p0.2 p.2) ;
+                        first (by specialize (injective_projections p0 p e) ; intro ;
+                                  rewrite -(nat_of_binK p0.2) -(nat_of_binK p.2) H0 in H1 ;
+                                  specialize (H1 Logic.eq_refl) ;
+                                  rewrite H1 eq_refl // in H21) ;
+                        first (by apply H9 ; right ; left  ; move /ltP : H0 => H0 ; exact H0) ;
+                  apply H9 ; right ; right ; move /ltP : H0 => H0 ; exact H0).
+        1,2: unfold code_type_find_vm_widths ;
+             rewrite H0 ;
+             fold (code_type_find_vm_widths (Gtyp gt0) p0 vm).
+        1,2: reflexivity.
+  rewrite H5 Hports_tmap in IHpp.
+  apply IHpp ; last by exact H4.
+  intro.
+  specialize (H3 v).
+  destruct (v == p) eqn: Hvp ; first by move /eqP : Hvp => Hvp ; rewrite Hvp Hfindp' //.
+  rewrite CEP.Lemmas.find_add_neq // in H3.
+  rewrite /PVM.SE.eq Hvp //.
 (* Second goal: similar, just that an element is added to ct. *)
-
-(* In both cases we would need somehow to include a property of ports_tmap in the inductive statement. *)
-
-
-
-
-(* Probably need something like: ports_tmap pp vm = Some pmap /\ submap pmap tmap *)
+* destruct H5 as [_ [H9 [H10 H11]]].
+  (*specialize (H5 0) ; rewrite /List.nth_error add0n nat_of_binK -surjective_pairing in H5.*)
+  intro.
+  specialize (H10 y.1 y.2) ; rewrite add1n -surjective_pairing in H10.
+  specialize (H11 0 is_true_true) ; rewrite add0n nat_of_binK -surjective_pairing in H11.
+  destruct (y == p) eqn: Hyp ;
+        first by (move /eqP : Hyp => Hyp ;
+                  rewrite CEP.Lemmas.find_add_eq /PVM.SE.eq Hyp // ;
+                  apply H11).
+  clear H11.
+  rewrite CEP.Lemmas.find_add_neq ; last by rewrite /PVM.SE.eq Hyp //.
+  assert (CEP.find y ct' = CEP.find y ct)
+        by (specialize (N.eq_dec y.1 p.1) ; intro ;
+            destruct H5 ; last (by apply H10 ; left ; exact n) ;
+            destruct (Nat.compare_spec y.2 p.2) ;
+                        first (by specialize (injective_projections y p e) ; intro ;
+                                  rewrite -(nat_of_binK y.2) -(nat_of_binK p.2) H5 in H11 ;
+                                  specialize (H11 Logic.eq_refl) ;
+                                  rewrite H11 eq_refl // in Hyp) ;
+                        first (by apply H10 ; right ; left  ; move /ltP : H5 => H5 ; exact H5) ;
+                  apply H10 ; right ; right ; move /ltP : H5 => H5 ; exact H5).
+  rewrite -H5 ; destruct H6 as [H6 _] ; clear ct H5 H10.
+  assert (ports_tmap pp vm' = ports_tmap pp vm).
+        clear -H2 H7 H9.
+        revert H2 H7.
+        induction pp ;
+              first by (unfold ports_tmap ; reflexivity).
+        intros ; simpl ports_tmap.
+        simpl ports_have_fully_inferred_ground_types in H7.
+        destruct a as [p0 [gt0| |]|p0 [gt0| |]] ; try done.
+        1,2: simpl uniq in H2 ; move /andP : H2 => [H21 /andP [_ H23]].
+        1,2: rewrite in_cons negb_or in H21.
+        1,2: move /andP : H21 => [H21 H22].
+        1,2: move /andP : H7 => [H H7].
+        1,2: simpl uniq in IHpp.
+        1,2: rewrite H22 H23 andTb in IHpp.
+        1,2: specialize (IHpp is_true_true H7).
+        1,2: rewrite IHpp.
+        1,2: assert (CEP.find p0 vm' = CEP.find p0 vm)
+              by (specialize (H9 p0.1 p0.2) ;
+                  rewrite add1n -surjective_pairing in H9 ;
+                  specialize (N.eq_dec p0.1 p.1) ; intro ;
+                  destruct H0 ; last (by apply H9 ; left ; exact n) ;
+                  destruct (Nat.compare_spec p0.2 p.2) ;
+                        first (by specialize (injective_projections p0 p e) ; intro ;
+                                  rewrite -(nat_of_binK p0.2) -(nat_of_binK p.2) H0 in H1 ;
+                                  specialize (H1 Logic.eq_refl) ;
+                                  rewrite H1 eq_refl // in H21) ;
+                        first (by apply H9 ; right ; left  ; move /ltP : H0 => H0 ; exact H0) ;
+                  apply H9 ; right ; right ; move /ltP : H0 => H0 ; exact H0).
+        1,2: unfold code_type_find_vm_widths ;
+             rewrite H0 ;
+             fold (code_type_find_vm_widths (Gtyp gt0) p0 vm).
+        1,2: reflexivity.
+  rewrite H5 Hports_tmap in IHpp.
+  apply IHpp ; last by exact H4.
+  intro.
+  specialize (H3 v).
+  destruct (v == p) eqn: Hvp ; first by move /eqP : Hvp => Hvp ; rewrite Hvp Hfindp' //.
+  rewrite CEP.Lemmas.find_add_neq // in H3.
+  rewrite /PVM.SE.eq Hvp //.
+Qed.
 
 (*
 Theorem ExpandBranch_Sem :
